[Progress] Finish extracting to non-FUSE version and add a tester client.

src/Extraction/Interpreter/Helpers.hs
@@ -1,0 +1,70 @@
+module Helpers where
+
+import Prelude
+import qualified Data.Bits
+import qualified Data.Word
+import qualified Data.Char
+import qualified Data.ByteArray as BA
+import qualified Data.ByteString as BS
+import qualified Data.ByteString.Lazy as BSL
+import qualified Data.Serialize as BIN
+import qualified Data.List.Split as L
+import qualified Data.Text as T
+import Data.Text.Encoding (encodeUtf8, decodeUtf8)
+
+intSize :: Int
+intSize = Data.Bits.finiteBitSize (1::Int)
+
+toBits :: Data.Word.Word8 -> [Bool]
+toBits x = [Data.Bits.testBit x i | i <- [0.. Data.Bits.finiteBitSize x - 1] ]
+
+toByte :: [Bool] -> Data.Word.Word8
+toByte list = toByteRec list 0 0
+
+toByteRec :: [Bool] -> Int -> Data.Word.Word8 -> Data.Word.Word8
+toByteRec list 8 result = result
+toByteRec list i result 
+    | head list == True = toByteRec (tail list) (i + 1) (result Data.Bits..|. (2^i :: Data.Word.Word8))
+    | otherwise = toByteRec (tail list) (i + 1) result
+
+byteStringToBoolList :: BS.ByteString -> [Bool]
+byteStringToBoolList bs =
+  concatMap toBits (BS.unpack bs)
+
+boolListToByteString :: [Bool] -> BS.ByteString 
+boolListToByteString  bl =
+  BS.pack (map toByte (L.chunksOf 8 bl))
+
+
+toByteString :: BA.ByteArrayAccess a => a -> BS.ByteString
+toByteString = BS.pack . BA.unpack
+
+setToBlockSize:: Int -> BS.ByteString -> BS.ByteString
+setToBlockSize bytesPerBlock bs 
+  | (BS.length bs) < bytesPerBlock = BS.append bs (BS.replicate (bytesPerBlock - BS.length bs) 0)
+  | otherwise = BS.take bytesPerBlock bs
+
+stringToBlock :: Int -> String -> BS.ByteString
+stringToBlock len str = (setToBlockSize len . encodeUtf8 . T.pack) str
+
+blockToString :: BS.ByteString -> String
+blockToString bs = (T.unpack . (T.takeWhile Data.Char.isPrint) . decodeUtf8) bs
+
+--written by Baricus
+
+padList :: Int -> [Int] -> [Int]
+padList intsPerBlock l | length l `mod` intsPerBlock == 0 = l
+          | otherwise = let addend = intsPerBlock - length l `mod` intsPerBlock in l ++ replicate addend 0
+
+intListToByteStringList :: Int -> [Int] -> [BS.ByteString]
+intListToByteStringList intsPerBlock list = map (BS.drop 8 . BIN.encode) $ (L.chunksOf intsPerBlock . padList intsPerBlock) list
+
+decodeChunk :: BS.ByteString -> [Int]
+decodeChunk bytes | BS.null bytes = []
+                  | otherwise = let (n, rest) = BS.splitAt (fromIntegral $ Data.Bits.finiteBitSize (1 :: Int) `div` 8) bytes
+                        in (case BIN.decode n of
+                          Left _ -> 0
+                          Right i -> i) : decodeChunk rest
+
+byteStringListToIntList :: [BS.ByteString] -> [Int]
+byteStringListToIntList = concatMap (decodeChunk)
