src/Extraction/Interpreter/Interpreter.hs
@@ -1,0 +1,111 @@
+{-# LANGUAGE PackageImports #-}
+module Interpreter where
+
+import Prelude
+import BaseTypes
+import Helpers
+import Crypto.Hash
+import Crypto.Hash.Algorithms
+import Data.IORef
+import "cipher-aes" Crypto.Cipher.AES
+import Data.Map
+import System.Random
+import System.Random.Stateful
+import System.IO
+import System.IO.Unsafe
+import qualified Data.ByteString as BS
+import Data.ByteString.Random
+import qualified Data.ByteArray
+
+
+
+addrsPerBlock :: Int
+addrsPerBlock = div block_size intSize 
+
+cache :: IORef (Map Coq_addr Coq_value)
+{-# NOINLINE cache #-}
+cache = unsafePerformIO (newIORef empty)
+
+txnList :: IORef [(Coq_addr, Coq_value)]
+{-# NOINLINE txnList #-}
+txnList = unsafePerformIO (newIORef [])
+
+-- Haskell doesn't allow us to access the key explicitly. 
+-- You get to initialize by giving a seed. 
+-- What I will do is keep 32-bit random seeds as "keys" in the header
+-- then initialize the cipherMap as it accesses. 
+cipherMap :: IORef (Map Coq_key AES)
+{-# NOINLINE cipherMap #-}
+cipherMap = unsafePerformIO (newIORef empty)
+
+getCipher :: Coq_key -> IO AES
+getCipher k = do
+  cm <- readIORef cipherMap
+  case (Data.Map.lookup k cm) of
+    Just c -> return c
+    Nothing -> 
+      do
+      let newCipher = initAES k
+      _ <- writeIORef cipherMap (insert k newCipher cm)
+      return newCipher
+
+
+fsImage :: Handle
+{-# NOINLINE fsImage #-}
+fsImage = unsafePerformIO (openBinaryFile "fs_image" ReadWriteMode)
+
+-- Disk Operations
+diskRead :: Coq_addr -> IO Coq_value
+diskRead a = --return BaseTypes.value0
+  do 
+  hSeek fsImage AbsoluteSeek (fromIntegral(4096 Prelude.* a))
+  BS.hGet fsImage 4096
+
+diskWrite :: Coq_addr -> Coq_value -> IO ()
+diskWrite a v = --return ()
+  do
+  hSeek fsImage AbsoluteSeek (fromIntegral(4096 Prelude.* a))
+  BS.hPut fsImage v
+
+diskSync :: IO ()
+diskSync = --return ()
+  hFlush fsImage
+
+-- Cache Operations
+cacheRead :: Coq_addr -> IO (Maybe Coq_value)
+cacheRead a = do 
+  c <- readIORef cache
+  return (Data.Map.lookup a c)
+
+cacheWrite :: Coq_addr -> Coq_value -> IO ()
+cacheWrite a v = modifyIORef' cache (insert a v)
+
+cacheFlush :: IO ()
+cacheFlush = writeIORef cache empty
+
+-- List Operations
+listGet :: IO [(Coq_addr , Coq_value)]
+listGet = readIORef txnList
+
+listPut :: (Coq_addr , Coq_value) -> IO ()
+listPut av = modifyIORef' txnList ((:) av)
+
+listDelete :: IO ()
+listDelete = writeIORef txnList []
+
+-- Crypto Operations
+cryptoHash :: Coq_hash -> Coq_value -> IO Coq_hash
+cryptoHash h v = return (toByteString (hash (BS.append h v) :: Digest MD5))
+
+cryptoGetKey :: IO Coq_key
+cryptoGetKey = uniformByteStringM 32 globalStdGen
+
+cryptoEncrypt :: Coq_key -> Coq_value -> IO Coq_value
+cryptoEncrypt k v = do 
+  cipher <- getCipher k;
+  return (encryptECB cipher v)
+
+cryptoDecrypt :: Coq_key -> Coq_value -> IO Coq_value
+cryptoDecrypt k v = do 
+    cipher <- getCipher k;
+    return (decryptECB cipher v)
