src/Extraction/Interpreter/Tester.hs
@@ -1,0 +1,80 @@
+import Prelude
+import Helpers
+import qualified File
+import qualified BaseTypes
+import qualified Data.ByteString as BS
+import qualified Data.ByteString.Lazy as BSL
+import qualified Data.Serialize as BIN
+import qualified Data.List.Split as L
+import System.Posix.Types
+import System.Posix.User
+import Data.Maybe
+
+repeatNTimes 0 _ = return ()
+repeatNTimes n action =
+ do
+  action n
+  repeatNTimes (n-1) action
+
+
+main :: IO ()
+main = do 
+{-
+    let l = replicate 2000 128
+    let intsPerBlock = div BaseTypes.block_size Helpers.intSize
+    print (padList intsPerBlock l)
+    print ((L.chunksOf intsPerBlock . padList intsPerBlock) l)
+    print (map (BS.length . BIN.encode) $ (L.chunksOf intsPerBlock . padList intsPerBlock) l)
+    print (map BS.length (BaseTypes.addr_list_to_blocks l))
+    print (BaseTypes.blocks_to_addr_list (BaseTypes.addr_list_to_blocks l))
+-}
+
+  do
+    File.init
+    userId <- getEffectiveUserID
+    fn <- File.create userId
+    print fn
+    let fileName = fromJust fn
+    repeatNTimes 510 (\ i ->  File.extend fileName (stringToBlock (div BaseTypes.block_size 8) "I love you <3"))
+    repeatNTimes 510 (\ i -> do
+      dat <- File.read fileName (i-1)
+      print ((blockToString . fromJust) dat))
+
+    File.write fileName 0 (stringToBlock (div BaseTypes.block_size 8) "Goodbye World!")
+    dat <- File.read fileName 0
+    print ((blockToString . fromJust) dat)
+
+    ret <- File.delete fileName
+    print (isJust ret)
+    dat <- File.read fileName 0
+    print (isNothing dat) --Should fail
+  
+    fn <- File.create userId
+    print fn
+    fa <- File.create (CUid 123)
+    print fa
+    let fileName = fromJust fn
+    dat <- File.read fileName 0
+    print (isNothing dat) --should fail
+
+    File.extend fileName (stringToBlock (div BaseTypes.block_size 8) "")
+    dat <- File.read fileName 0
+    print ((blockToString . fromJust) dat)
+
+    ret <- File.change_owner fileName userId
+    print (isJust ret) --should succeed
+    dat <- File.read fileName 0
+    print ((blockToString . fromJust) dat)
+
+    ret <- File.change_owner fileName (CUid 123)
+    print (isJust ret)
+
+    dat <- File.read fileName 0
+    print (isNothing dat) --should fail
+
+    ret <- File.change_owner fileName userId
+    print (isNothing dat) --should fail
+
+    fn <- File.create userId
+    print fn
+    return ()
