src/Implementations/BatchOperations/BatchOperations.v
@@ -327,3 +327,223 @@ Qed.
 
 Definition write_consecutive_finished := write_batch_finished.
 Definition write_consecutive_crashed := write_batch_crashed.
+
+
+Theorem encrypt_all_finished_oracle:
+  forall key vl o s s' t u,
+    exec CryptoDiskLang u o s (encrypt_all key vl) (Finished s' t) ->
+    t = map (encrypt key) vl /\
+    consistent_with_upds (snd (fst s)) (map (encrypt key) vl) (map (fun v => (key, v)) vl) /\
+    fst (fst s') = fst (fst s) /\
+    snd (fst s') = upd_batch (snd (fst s)) (map (encrypt key) vl) (map (fun v => (key, v)) vl) /\
+    snd s' = snd s /\
+    (length o = S (length vl + length vl)).
+Proof.
+  induction vl; simpl; intros;
+  cleanup; simpl in *; repeat invert_exec;
+  cleanup; try lia; simpl; eauto.
+  - intuition eauto.
+  - edestruct IHvl; eauto; cleanup.
+    eexists; intuition eauto.
+    repeat cleanup_pairs; eauto.
+    rewrite app_length; simpl.
+    setoid_rewrite H5; simpl. 
+    lia.
+Qed.
+
+Theorem encrypt_all_crashed_oracle:
+  forall key vl o s s' u,
+    exec CryptoDiskLang u o s (encrypt_all key vl) (Crashed s') ->
+    exists n,
+      consistent_with_upds (snd (fst s)) (firstn n (map (encrypt key) vl)) (firstn n (map (fun v => (key, v)) vl)) /\
+      fst (fst s') = fst (fst s) /\
+      snd (fst s') = upd_batch (snd (fst s)) (firstn n (map (encrypt key) vl)) (firstn n (map (fun v => (key, v)) vl)) /\
+      snd s' = snd s /\
+      n <= length vl + length vl /\
+      S n = length o.
+Proof.
+  induction vl; simpl; intros;
+  cleanup_no_match; simpl in *; 
+  repeat invert_exec_no_match;
+  cleanup_no_match; try lia; eauto.
+  {
+    exists 0; simpl; intuition eauto.
+  }
+  split_ors; cleanup_no_match; 
+  repeat invert_exec_no_match.
+  {
+    exists 0; simpl; intuition eauto.
+    lia.
+  }
+  split_ors; cleanup_no_match; 
+  repeat invert_exec_no_match.
+  {
+    eapply IHvl in H; eauto;
+    cleanup_no_match; 
+    eauto; simpl.
+    exists (S x); simpl; cleanup_no_match; intuition eauto;
+    repeat cleanup_pairs; eauto;
+    destruct p; simpl in *; eauto; try lia.
+  }
+  {
+    eapply encrypt_all_finished_oracle in H0; cleanup_no_match.
+
+    exists (S(S (length vl + length vl))); intuition eauto;
+    repeat rewrite firstn_oob; simpl; eauto;
+    try solve [rewrite map_length; simpl; lia];
+    repeat cleanup_pairs; eauto.
+    destruct p; simpl; eauto.
+
+    lia.
+    rewrite app_length; simpl.
+    setoid_rewrite H4; simpl.
+    lia.
+  }      
+Qed.
+
+Theorem hash_all_finished_oracle:
+  forall vl h o s t s' u,
+    exec CryptoDiskLang u o s (hash_all h vl) (Finished s' t) ->
+    t = rolling_hash h vl /\
+    consistent_with_upds (snd (fst (fst s))) (rolling_hash_list h vl) (combine (h:: rolling_hash_list h vl) vl) /\
+    (snd (fst (fst s'))) = upd_batch (snd (fst (fst s))) (rolling_hash_list h vl) (combine (h:: rolling_hash_list h vl) vl) /\
+    fst (fst (fst s')) = fst (fst (fst s)) /\
+    snd (fst s') = snd (fst s) /\
+    snd s' = snd s /\
+    length o = S (length vl + length vl).
+Proof.
+  induction vl; simpl; intros.
+  repeat invert_exec; cleanup; intuition eauto.
+  repeat invert_exec; cleanup.
+  edestruct IHvl; eauto; cleanup.
+  simpl in *; intuition eauto.
+  rewrite app_length; simpl.
+  setoid_rewrite H6; lia.
+Qed.
+
+Lemma rolling_hash_list_length :
+forall l h,
+length (rolling_hash_list h l) = length l.
+Proof.
+  induction l; simpl; intuition eauto.
+Qed.
+
+Theorem hash_all_crashed_oracle:
+  forall vl h o s s' u,
+    exec CryptoDiskLang u o s (hash_all h vl) (Crashed s') ->
+    exists n,
+      n <= length (rolling_hash_list h vl) /\
+    consistent_with_upds (snd (fst (fst s))) (firstn n (rolling_hash_list h vl)) (firstn n (combine (h:: rolling_hash_list h vl) vl)) /\
+    (snd (fst (fst s'))) = upd_batch (snd (fst (fst s))) (firstn n (rolling_hash_list h vl)) (firstn n (combine (h:: rolling_hash_list h vl) vl)) /\
+    fst (fst (fst s')) = fst (fst (fst s)) /\
+    snd (fst s') = snd (fst s) /\
+    snd s' = snd s /\
+    length o <= S (n + n).
+Proof.
+  induction vl; simpl; intros.
+  repeat invert_exec; cleanup; simpl; eauto.
+  exists 0; simpl; intuition eauto.
+  
+  repeat invert_exec; cleanup.
+  repeat (split_ors; cleanup; repeat invert_exec; simpl; eauto).
+  exists 0; simpl; intuition eauto.
+  lia.
+  
+  edestruct IHvl; eauto; cleanup.
+  simpl in *; repeat cleanup_pairs; eauto.
+  exists (S x); simpl; intuition eauto.
+  lia.
+  lia.
+    
+  eapply hash_all_finished_oracle in H0; cleanup; eauto;
+  simpl in *; intuition eauto.
+  repeat cleanup_pairs; eauto.
+  exists (length (hash_function h a :: rolling_hash_list (hash_function h a) vl)).
+  repeat rewrite firstn_oob;
+  simpl; intuition eauto.
+ 
+  repeat rewrite rolling_hash_list_length, app_length.
+  simpl.
+  setoid_rewrite H5; lia.
+
+  generalize vl (hash_function h a).
+  induction vl0; simpl; intros; eauto.
+  destruct vl0; simpl in *; eauto.
+  specialize (IHvl0 (hash_function h1 a0)); lia.
+Qed.
+
+
+Theorem write_batch_finished_oracle:
+  forall al vl o t s s' u,
+    length al = length vl ->
+    exec CryptoDiskLang u o s (write_batch al vl) (Finished s' t) ->
+    (forall a, In a al -> a < disk_size) /\
+    fst s' = fst s /\ snd s' = TotalMem.upd_batch_set (snd s) al vl /\
+    length o = S (length al + length al).
+Proof.
+  induction al; simpl; intros;
+  cleanup; simpl in *; repeat invert_exec;
+  cleanup; try lia; eauto.
+  intuition eauto.
+
+  eapply IHal in H0; try lia; cleanup.
+  simpl in *; cleanup.
+  intuition eauto.
+  subst; congruence.
+  rewrite app_length; simpl.
+  setoid_rewrite H3; lia.
+Qed.
+
+Theorem write_batch_crashed_oracle:
+  forall al vl o s s' u,
+    length al = length vl ->
+    exec CryptoDiskLang u o s (write_batch al vl) (Crashed s') ->
+    exists n,
+      n <= length al /\
+      (forall a, In a (firstn n al) -> a < disk_size) /\
+      fst s' = fst s /\ 
+      snd s' = TotalMem.upd_batch_set (snd s) (firstn n al) (firstn n vl) /\
+      length o > 0 /\
+      length o <= S (n + n).
+Proof.
+  induction al; simpl; intros;
+  cleanup; simpl in *; repeat invert_exec;
+  cleanup; try lia; eauto.
+  {
+    exists 0; split; intuition eauto.
+    simpl in *; intuition.
+  }
+  
+  split_ors; cleanup; repeat invert_exec; simpl.
+  {
+    exists 0; split; intuition eauto; simpl in *.
+    lia.
+    intuition.
+  }
+
+  split_ors; cleanup; repeat invert_exec; simpl in *.
+  {
+    eapply IHal in H0; try lia.
+    cleanup; simpl in *; cleanup.
+    exists (S x); split; intuition eauto; simpl in *.
+    lia.
+    split_ors; cleanup; eauto.
+    lia.
+  }
+  {
+    eapply write_batch_finished_oracle in H1; eauto; cleanup.
+    simpl in *; cleanup.
+    exists (S (length al)).
+    simpl.
+    repeat rewrite firstn_oob by lia.
+    cleanup; split; intuition eauto; simpl in *.
+    cleanup.
+    eauto.
+    lia.
+    rewrite app_length; simpl.
+    setoid_rewrite H3; lia.
+  }
+Qed.
+
+Definition write_consecutive_finished_oracle := write_batch_finished_oracle.
+Definition write_consecutive_crashed_oracle := write_batch_crashed_oracle.
