src/Extraction/Extraction.v
@@ -11,41 +11,54 @@ Require Import ExtrHaskellString.
 
 Extraction Language Haskell.
 
-
-
 Require Import Framework FSParameters.
-Require LogCache Transaction File.
+Require LogCache Transaction BlockAllocator File.
 
 (** Write to a file to test the system **)
-Extract Constant addr => "Prelude.Int".
+Extract Constant addr => "Int".
 Extract Inlined Constant addr_eq_dec => "(Prelude.==)".
 
 Extract Constant user => "System.Posix.Types.UserID".
-Extract Constant value => "Data.ByteArray.Sized 4096".
-Extract Constant block_size => "8 Prelude.* 4096". (** 4KB blocks **) 
+Extract Constant value => "Data.ByteString.ByteString".
+Extract Constant block_size => "8 * 4096". (** 4KB blocks **)
+Extract Constant value0 => "Data.ByteString.pack (Data.List.replicate (div block_size 8) (0::Data.Word.Word8))".
 Extract Constant file_blocks_count => "4096". (** 4K data blocks *)
-Extract Constant log_length => "500". (** 500 log blocks *)
+Extract Constant log_length => "600". (** 500 log blocks *)
 Extract Constant inode_count => "4096". (** 4K inodes *)
-Extract Constant disk_size => "4 Prelude.* 1024 Prelude.* 1024 Prelude.* 1024". (** 4 GB disk *)
+Extract Constant disk_size => "4 * 1024 * 1024 * 1024". (** 4 GB disk *)
 
-(** These need to be defined as well
-Extract Constant BlockAllocator.bits_to_value => "".
-Extract Constant BlockAllocator.value_to_bits => "".
 
-Extract Constant addr_list_to_blocks => "".
-Extract Constant blocks_to_addr_list => "".
+Extract Constant addr_list_to_blocks => 
+"Helpers.intListToByteStringList (div block_size Helpers.intSize)".
 
-Extract Constant Log.encode_header => "".
-Extract Constant Log.decode_header => "".
+Extract Constant blocks_to_addr_list => 
+"Helpers.byteStringListToIntList".
 
-Extract Constant hash => "".
-Extract Inline Constant hash_eq_dec => "".
-Extract Inline Constant hash0 => "".
+Extract Constant hash => "Data.ByteString.ByteString".
+Extract Constant hash0 => "Helpers.toByteString (Crypto.Hash.hash value0 :: Crypto.Hash.Digest Crypto.Hash.Algorithms.MD5)".
+Extract Constant hash_eq_dec => "(Prelude.==)".
 
-Extract Constant key => "".
-Extract Constant Inode.encode_inode => "".
-Extract Constant Inode.decode_inode => "".
-**)
+Extract Constant key => "Data.ByteString.ByteString".
+
+Extract Constant value_to_bits =>
+"Helpers.byteStringToBoolList".
+
+Extract Constant bits_to_value =>
+"Helpers.boolListToByteString".
+
+(** These need to be defined as well **)
+Extract Constant Log.encode_header => "(Helpers.setToBlockSize (Prelude.div BaseTypes.block_size 8) Prelude.. Data.Serialize.encode)".
+Extract Constant Log.decode_header =>
+"\x -> case Data.Serialize.decode x of 
+Prelude.Left _ -> header0; 
+Prelude.Right h -> h".
+
+Extract Constant Inode.encode_inode => "(Helpers.setToBlockSize (Prelude.div BaseTypes.block_size 8) Prelude.. Data.Serialize.encode)".
+Extract Constant Inode.decode_inode =>
+"\x -> case Data.Serialize.decode x of 
+Prelude.Left _ -> Build_Inode 0 []; 
+Prelude.Right h -> h".
+
 
 (** Eliminate Horizontal Composition **) 
 Extraction Implicit lift_L1 [ 1 2 ].
@@ -61,17 +74,10 @@ Extract Inductive Language.prog' => "Prelude.IO" [ "" "Prelude.return" "(Prelude
 (** Using file as a disk *)
 
 Extract Inductive DiskLayer.disk_prog => "Prelude.IO" [ "Interpreter.diskRead" "Interpreter.diskWrite" "Interpreter.diskSync" ].
-Extract Inductive CryptoLayer.crypto_prog => "Prelude.IO" [ "GET_KEY" "HASH" "ENCRYPT" "DECRYPT" ].
+Extract Inductive CryptoLayer.crypto_prog => "Prelude.IO" [ "Interpreter.cryptoGetKey" "Interpreter.cryptoHash" "Interpreter.cryptoEncrypt" "Interpreter.cryptoDecrypt" ].
 Extract Inductive CacheLayer.cache_prog => "Prelude.IO" [ "Interpreter.cacheRead" "Interpreter.cacheWrite" "Interpreter.cacheFlush"]. 
 Extract Inductive ListLayer.list_prog => "Prelude.IO" [ "Interpreter.listGet" "Interpreter.listPut" "Interpreter.listDelete" ].
 
-
-(** Use these to implement actual functionality 
-Extract Inductive DiskLayer.disk_prog => "Prelude.IO" [ "DISK_READ" "DISK_WRITE" "DISK_SYNC" ].
-Extract Inductive CryptoLayer.crypto_prog => "Prelude.IO" [ "GET_KEY" "HASH" "ENCRYPT" "DECRYPT" ].
-Extract Inductive CacheLayer.cache_prog => "Prelude.IO" [ "CACHE_READ" "CACHE_WRITE" "CACHE_FLUSH"]. 
-Extract Inductive ListLayer.list_prog => "Prelude.IO" [ "GET" "PUT" "DELETE" ].
-*)
 
 Extract Inductive AuthenticationLayer.authentication_prog =>
 "Prelude.IO" [ "(\u -> do uid <- System.Posix.User.getEffectiveUserID; Prelude.return (u Prelude.== uid))" ].
