src/Noninterference/LoggedDisk/ATCD_TIE.v
@@ -14,6 +14,19 @@ match goal with
   destruct x
 end.
 
+Ltac solve_get_first:=
+  unfold AD_related_states, refines_related in *; simpl in *; cleanup;
+  unfold refines, File.files_rep in *; simpl in *; cleanup;
+  unfold HC_refines in *; simpl in *; cleanup;
+  unfold TransactionToTransactionalDisk.Definitions.refines,
+  Transaction.transaction_rep in *; simpl in *; cleanup;
+  repeat split_ors; cleanup; try congruence;
+  repeat cleanup_pairs;
+  match goal with
+  | [|- Transaction.get_first ?s _ = _ ] =>
+    destruct s; simpl in *; try lia; eauto
+  end.
+
 
 Lemma TIE_auth_then_exec:
     forall T (p1 p2: addr -> TD.(prog) (option T)) inum s1 s2 u ex,
@@ -39,27 +52,8 @@ Lemma TIE_auth_then_exec:
       Inode.InodeAllocatorParams.num_of_blocks);
       destruct (Compare_dec.lt_dec inum
       Inode.InodeAllocatorParams.num_of_blocks); simpl; intuition eauto.
-      
-      {
-        unfold AD_related_states, refines_related in *; simpl in *; cleanup.
-        unfold refines, File.files_rep in *; simpl in *; cleanup.
-        unfold HC_refines in *; simpl in *; cleanup.
-        unfold TransactionToTransactionalDisk.Definitions.refines,
-        Transaction.transaction_rep in *; simpl in *; cleanup.
-        repeat split_ors; cleanup; try congruence.
-        repeat cleanup_pairs.
-        destruct s, s0; simpl in *; try lia; eauto.
-      }
-      {
-        unfold AD_related_states, refines_related in *; simpl in *; cleanup.
-        unfold refines, File.files_rep in *; simpl in *; cleanup.
-        unfold HC_refines in *; simpl in *; cleanup.
-        unfold TransactionToTransactionalDisk.Definitions.refines,
-        Transaction.transaction_rep in *; simpl in *; cleanup.
-        repeat split_ors; cleanup; try congruence.
-        repeat cleanup_pairs.
-        destruct s, s0; simpl in *; try lia; eauto.
-      }
+      solve_get_first.
+      solve_get_first.
       unfold HC_refines in *; simpl in *; cleanup.
       unfold TransactionToTransactionalDisk.Definitions.refines in *; simpl in *; cleanup.
       repeat invert_lift2; cleanup.
@@ -70,26 +64,8 @@ Lemma TIE_auth_then_exec:
       destruct (nth_error (value_to_bits r2) inum);
       simpl; intuition eauto.
       destruct b, b0; simpl; intuition eauto.
-      {
-        unfold AD_related_states, refines_related in *; simpl in *; cleanup.
-        unfold refines, File.files_rep in *; simpl in *; cleanup.
-        unfold HC_refines in *; simpl in *; cleanup.
-        unfold TransactionToTransactionalDisk.Definitions.refines,
-        Transaction.transaction_rep in *; simpl in *; cleanup.
-        repeat split_ors; cleanup; try congruence.
-        repeat cleanup_pairs.
-        destruct s, s0; simpl in *; try lia; eauto.
-      }
-      {
-        unfold AD_related_states, refines_related in *; simpl in *; cleanup.
-        unfold refines, File.files_rep in *; simpl in *; cleanup.
-        unfold HC_refines in *; simpl in *; cleanup.
-        unfold TransactionToTransactionalDisk.Definitions.refines,
-        Transaction.transaction_rep in *; simpl in *; cleanup.
-        repeat split_ors; cleanup; try congruence.
-        repeat cleanup_pairs.
-        destruct s, s0; simpl in *; try lia; eauto.
-      }
+      solve_get_first.
+      solve_get_first.
       destruct b; simpl; intuition eauto.
       all: repeat destruct_and_split; simpl; eauto.
       Opaque Inode.get_owner.
@@ -169,27 +145,8 @@ Proof.
     Inode.InodeAllocatorParams.num_of_blocks);
     destruct (Compare_dec.lt_dec inum
     Inode.InodeAllocatorParams.num_of_blocks); simpl; intuition eauto.
-    
-    {
-      unfold AD_related_states, refines_related in *; simpl in *; cleanup.
-      unfold refines, File.files_rep in *; simpl in *; cleanup.
-      unfold HC_refines in *; simpl in *; cleanup.
-      unfold TransactionToTransactionalDisk.Definitions.refines,
-      Transaction.transaction_rep in *; simpl in *; cleanup.
-      repeat split_ors; cleanup; try congruence.
-      repeat cleanup_pairs.
-      destruct s, s1; simpl in *; try lia; eauto.
-    }
-    {
-      unfold AD_related_states, refines_related in *; simpl in *; cleanup.
-      unfold refines, File.files_rep in *; simpl in *; cleanup.
-      unfold HC_refines in *; simpl in *; cleanup.
-      unfold TransactionToTransactionalDisk.Definitions.refines,
-      Transaction.transaction_rep in *; simpl in *; cleanup.
-      repeat split_ors; cleanup; try congruence.
-      repeat cleanup_pairs.
-      destruct s, s1; simpl in *; try lia; eauto.
-      }
+    solve_get_first.
+    solve_get_first.
       unfold HC_refines in *; simpl in *; cleanup.
       unfold TransactionToTransactionalDisk.Definitions.refines in *; simpl in *; cleanup.
       repeat invert_lift2; cleanup.
@@ -200,26 +157,8 @@ Proof.
       destruct (nth_error (value_to_bits r2) inum);
       simpl; intuition eauto.
       destruct b, b0; simpl; intuition eauto.
-      {
-        unfold AD_related_states, refines_related in *; simpl in *; cleanup.
-        unfold refines, File.files_rep in *; simpl in *; cleanup.
-        unfold HC_refines in *; simpl in *; cleanup.
-        unfold TransactionToTransactionalDisk.Definitions.refines,
-        Transaction.transaction_rep in *; simpl in *; cleanup.
-        repeat split_ors; cleanup; try congruence.
-        repeat cleanup_pairs.
-        destruct s, s1; simpl in *; try lia; eauto.
-      }
-      {
-        unfold AD_related_states, refines_related in *; simpl in *; cleanup.
-        unfold refines, File.files_rep in *; simpl in *; cleanup.
-        unfold HC_refines in *; simpl in *; cleanup.
-        unfold TransactionToTransactionalDisk.Definitions.refines,
-        Transaction.transaction_rep in *; simpl in *; cleanup.
-        repeat split_ors; cleanup; try congruence.
-        repeat cleanup_pairs.
-        destruct s, s1; simpl in *; try lia; eauto.
-      }
+      solve_get_first.
+      solve_get_first.
       destruct b; simpl; intuition eauto.
       all: repeat destruct_and_split; simpl; eauto.
       Opaque Inode.get_block_number.
@@ -260,27 +199,8 @@ Proof.
     destruct (Compare_dec.lt_dec
     (seln (Inode.block_numbers x4) off 0)
     File.DiskAllocatorParams.num_of_blocks); simpl; intuition eauto.
-    
-    {
-      unfold AD_related_states, refines_related in *; simpl in *; cleanup.
-      unfold refines, File.files_rep in *; simpl in *; cleanup.
-      unfold HC_refines in *; simpl in *; cleanup.
-      unfold TransactionToTransactionalDisk.Definitions.refines,
-      Transaction.transaction_rep in *; simpl in *; cleanup.
-      repeat split_ors; cleanup; try congruence.
-      repeat cleanup_pairs.
-      destruct s, s2; simpl in *; try lia; eauto.
-    }
-    {
-      unfold AD_related_states, refines_related in *; simpl in *; cleanup.
-      unfold refines, File.files_rep in *; simpl in *; cleanup.
-      unfold HC_refines in *; simpl in *; cleanup.
-      unfold TransactionToTransactionalDisk.Definitions.refines,
-      Transaction.transaction_rep in *; simpl in *; cleanup.
-      repeat split_ors; cleanup; try congruence.
-      repeat cleanup_pairs.
-      destruct s, s2; simpl in *; try lia; eauto.
-    }
+    solve_get_first.
+    solve_get_first.
       unfold HC_refines in *; simpl in *; cleanup.
       unfold TransactionToTransactionalDisk.Definitions.refines in *; simpl in *; cleanup.
       repeat invert_lift2; cleanup.
@@ -305,26 +225,8 @@ Proof.
         eapply File.DiskAllocator.block_allocator_rep_inbounds_eq; 
         [| intros; FileInnerSpecs.solve_bounds ]; eauto.
       }
-      {
-        unfold AD_related_states, refines_related in *; simpl in *; cleanup.
-        unfold refines, File.files_rep in *; simpl in *; cleanup.
-        unfold HC_refines in *; simpl in *; cleanup.
-        unfold TransactionToTransactionalDisk.Definitions.refines,
-        Transaction.transaction_rep in *; simpl in *; cleanup.
-        repeat split_ors; cleanup; try congruence.
-        repeat cleanup_pairs.
-        destruct s, s2; simpl in *; try lia; eauto.
-      }
-      {
-        unfold AD_related_states, refines_related in *; simpl in *; cleanup.
-        unfold refines, File.files_rep in *; simpl in *; cleanup.
-        unfold HC_refines in *; simpl in *; cleanup.
-        unfold TransactionToTransactionalDisk.Definitions.refines,
-        Transaction.transaction_rep in *; simpl in *; cleanup.
-        repeat split_ors; cleanup; try congruence.
-        repeat cleanup_pairs.
-        destruct s, s2; simpl in *; try lia; eauto.
-      }
+      solve_get_first.
+      solve_get_first.
       destruct b; simpl; intuition eauto.
     }
   }
@@ -335,7 +237,7 @@ Qed.
 
 
 Lemma TIE_write_inner:
-    forall off inum u s0 s3 v,
+    forall off inum u s0 s3 v1 v2,
 refines_related ATC_Refinement
 (fun s4 s5 : state AD =>
  exists s1a s2a : disk File,
@@ -345,8 +247,8 @@ refines_related ATC_Refinement
    File.files_inner_rep s2a (fst (snd (snd s5))) /\
    FD_related_states u None s1a s2a) s0 s3 ->
 transaction_input_equiv
-(@lift_L2 AuthenticationOperation _ TD _ (File.write_inner off v inum))
-(@lift_L2 AuthenticationOperation _ TD _ (File.write_inner off v inum)) s0 s3.
+(@lift_L2 AuthenticationOperation _ TD _ (File.write_inner off v1 inum))
+(@lift_L2 AuthenticationOperation _ TD _ (File.write_inner off v2 inum)) s0 s3.
 Proof.
       Transparent File.write_inner.  
       unfold refines_related, File.write_inner; simpl; intuition eauto; cleanup.
@@ -359,27 +261,8 @@ Proof.
     Inode.InodeAllocatorParams.num_of_blocks);
     destruct (Compare_dec.lt_dec inum
     Inode.InodeAllocatorParams.num_of_blocks); simpl; intuition eauto.
-    
-    {
-      unfold AD_related_states, refines_related in *; simpl in *; cleanup.
-      unfold refines, File.files_rep in *; simpl in *; cleanup.
-      unfold HC_refines in *; simpl in *; cleanup.
-      unfold TransactionToTransactionalDisk.Definitions.refines,
-      Transaction.transaction_rep in *; simpl in *; cleanup.
-      repeat split_ors; cleanup; try congruence.
-      repeat cleanup_pairs.
-      destruct s, s1; simpl in *; try lia; eauto.
-    }
-    {
-      unfold AD_related_states, refines_related in *; simpl in *; cleanup.
-      unfold refines, File.files_rep in *; simpl in *; cleanup.
-      unfold HC_refines in *; simpl in *; cleanup.
-      unfold TransactionToTransactionalDisk.Definitions.refines,
-      Transaction.transaction_rep in *; simpl in *; cleanup.
-      repeat split_ors; cleanup; try congruence.
-      repeat cleanup_pairs.
-      destruct s, s1; simpl in *; try lia; eauto.
-    }
+    solve_get_first.
+    solve_get_first.
     unfold HC_refines in *; simpl in *; cleanup.
     unfold TransactionToTransactionalDisk.Definitions.refines in *; simpl in *; cleanup.
     repeat invert_lift2; cleanup.
@@ -390,26 +273,8 @@ Proof.
     destruct (nth_error (value_to_bits r2) inum);
     simpl; intuition eauto.
     destruct b, b0; simpl; intuition eauto.
-    {
-      unfold AD_related_states, refines_related in *; simpl in *; cleanup.
-      unfold refines, File.files_rep in *; simpl in *; cleanup.
-      unfold HC_refines in *; simpl in *; cleanup.
-      unfold TransactionToTransactionalDisk.Definitions.refines,
-      Transaction.transaction_rep in *; simpl in *; cleanup.
-      repeat split_ors; cleanup; try congruence.
-      repeat cleanup_pairs.
-      destruct s, s1; simpl in *; try lia; eauto.
-    }
-    {
-      unfold AD_related_states, refines_related in *; simpl in *; cleanup.
-      unfold refines, File.files_rep in *; simpl in *; cleanup.
-      unfold HC_refines in *; simpl in *; cleanup.
-      unfold TransactionToTransactionalDisk.Definitions.refines,
-      Transaction.transaction_rep in *; simpl in *; cleanup.
-      repeat split_ors; cleanup; try congruence.
-      repeat cleanup_pairs.
-      destruct s, s1; simpl in *; try lia; eauto.
-    }
+    solve_get_first.
+    solve_get_first.
     destruct b; simpl; intuition eauto.
     all: repeat destruct_and_split; simpl; eauto.
     Opaque Inode.get_block_number.
@@ -450,27 +315,8 @@ Proof.
     destruct (Compare_dec.lt_dec
     (seln (Inode.block_numbers x4) off 0)
     File.DiskAllocatorParams.num_of_blocks); simpl; intuition eauto.
-    
-    {
-      unfold AD_related_states, refines_related in *; simpl in *; cleanup.
-      unfold refines, File.files_rep in *; simpl in *; cleanup.
-      unfold HC_refines in *; simpl in *; cleanup.
-      unfold TransactionToTransactionalDisk.Definitions.refines,
-      Transaction.transaction_rep in *; simpl in *; cleanup.
-      repeat split_ors; cleanup; try congruence.
-      repeat cleanup_pairs.
-      destruct s, s2; simpl in *; try lia; eauto.
-    }
-    {
-      unfold AD_related_states, refines_related in *; simpl in *; cleanup.
-      unfold refines, File.files_rep in *; simpl in *; cleanup.
-      unfold HC_refines in *; simpl in *; cleanup.
-      unfold TransactionToTransactionalDisk.Definitions.refines,
-      Transaction.transaction_rep in *; simpl in *; cleanup.
-      repeat split_ors; cleanup; try congruence.
-      repeat cleanup_pairs.
-      destruct s, s2; simpl in *; try lia; eauto.
-    }
+    solve_get_first.
+    solve_get_first.
       unfold HC_refines in *; simpl in *; cleanup.
       unfold TransactionToTransactionalDisk.Definitions.refines in *; simpl in *; cleanup.
       repeat invert_lift2; cleanup.
@@ -528,9 +374,9 @@ Qed.
 
 
 Lemma TIE_create:
-    forall u' s1 s2 v,
+    forall ex u' s1 s2 v,
 refines_related ATC_Refinement
-  (AD_related_states u' None) s1 s2 ->
+  (AD_related_states u' ex) s1 s2 ->
 transaction_input_equiv
 (File.create v) (File.create v) s1 s2.
 Proof.
@@ -540,26 +386,8 @@ unfold refines_related, File.create; simpl; intuition eauto; cleanup.
   Transparent Inode.alloc.
   unfold Inode.alloc.
   simpl; intuition eauto.
-  {
-    unfold AD_related_states, refines_related in *; simpl in *; cleanup.
-    unfold refines, File.files_rep in *; simpl in *; cleanup.
-    unfold HC_refines in *; simpl in *; cleanup.
-    unfold TransactionToTransactionalDisk.Definitions.refines,
-    Transaction.transaction_rep in *; simpl in *; cleanup.
-    repeat split_ors; cleanup; try congruence.
-    repeat cleanup_pairs.
-    destruct s, s0; simpl in *; try lia; eauto.
-  }
-  {
-    unfold AD_related_states, refines_related in *; simpl in *; cleanup.
-    unfold refines, File.files_rep in *; simpl in *; cleanup.
-    unfold HC_refines in *; simpl in *; cleanup.
-    unfold TransactionToTransactionalDisk.Definitions.refines,
-    Transaction.transaction_rep in *; simpl in *; cleanup.
-    repeat split_ors; cleanup; try congruence.
-    repeat cleanup_pairs.
-    destruct s, s0; simpl in *; try lia; eauto.
-  }
+  solve_get_first.
+  solve_get_first.
   unfold HC_refines in *; simpl in *; cleanup.
   unfold TransactionToTransactionalDisk.Definitions.refines in *; simpl in *; cleanup.
   repeat invert_lift2; cleanup.
@@ -648,7 +476,7 @@ repeat destruct_and_split; simpl; intuition eauto.
 Qed.
 
 Lemma TIE_extend_inner:
-    forall inum u s0 s3 v,
+    forall inum ex u s0 s3 v1 v2,
 refines_related ATC_Refinement
 (fun s4 s5 : state AD =>
  exists s1a s2a : disk File,
@@ -656,10 +484,10 @@ refines_related ATC_Refinement
  fst (snd s5) = Empty /\
    File.files_inner_rep s1a (fst (snd (snd s4))) /\
    File.files_inner_rep s2a (fst (snd (snd s5))) /\
-   FD_related_states u None s1a s2a) s0 s3 ->
+   FD_related_states u ex s1a s2a) s0 s3 ->
 transaction_input_equiv
-(@lift_L2 AuthenticationOperation _ TD _ (File.extend_inner v inum))
-(@lift_L2 AuthenticationOperation _ TD _ (File.extend_inner v inum)) s0 s3.
+(@lift_L2 AuthenticationOperation _ TD _ (File.extend_inner v1 inum))
+(@lift_L2 AuthenticationOperation _ TD _ (File.extend_inner v2 inum)) s0 s3.
 Proof.
   Transparent File.extend_inner.  
   Opaque File.DiskAllocator.alloc.
@@ -667,26 +495,8 @@ Proof.
 {
   Transparent File.DiskAllocator.alloc.
   simpl; intuition eauto.
-  {
-    unfold AD_related_states, refines_related in *; simpl in *; cleanup.
-    unfold refines, File.files_rep in *; simpl in *; cleanup.
-    unfold HC_refines in *; simpl in *; cleanup.
-    unfold TransactionToTransactionalDisk.Definitions.refines,
-    Transaction.transaction_rep in *; simpl in *; cleanup.
-    repeat split_ors; cleanup; try congruence.
-    repeat cleanup_pairs.
-    destruct s, s1; simpl in *; try lia; eauto.
-  }
-  {
-    unfold AD_related_states, refines_related in *; simpl in *; cleanup.
-    unfold refines, File.files_rep in *; simpl in *; cleanup.
-    unfold HC_refines in *; simpl in *; cleanup.
-    unfold TransactionToTransactionalDisk.Definitions.refines,
-    Transaction.transaction_rep in *; simpl in *; cleanup.
-    repeat split_ors; cleanup; try congruence.
-    repeat cleanup_pairs.
-    destruct s, s1; simpl in *; try lia; eauto.
-  }
+  solve_get_first.
+  solve_get_first.
 
   unfold HC_refines in *; simpl in *; cleanup.
   unfold TransactionToTransactionalDisk.Definitions.refines in *; simpl in *; cleanup.
@@ -770,7 +580,6 @@ Proof.
 }
 repeat destruct_and_split; simpl; intuition eauto.
 {
-   (***********)
    unfold HC_refines in *; simpl in *; cleanup.
     unfold TransactionToTransactionalDisk.Definitions.refines in *; simpl in *; cleanup.
     unfold File.DiskAllocator.alloc in *; simpl in *.
@@ -946,4 +755,714 @@ repeat destruct_and_split; simpl; intuition eauto.
       File.DiskAllocatorParams.bitmap_addr,
       Inode.InodeAllocatorParams.num_of_blocks in *;
       pose proof inodes_before_data; try lia.
+Qed.
+
+Lemma TIE_change_owner_inner:
+forall inum ex u s0 s3 v,
+refines_related ATC_Refinement
+(fun s4 s5 : state AD =>
+ exists s1a s2a : disk File,
+ fst (snd s4) = Empty /\
+ fst (snd s5) = Empty /\
+   File.files_inner_rep s1a (fst (snd (snd s4))) /\
+   File.files_inner_rep s2a (fst (snd (snd s5))) /\
+   FD_related_states u ex s1a s2a) s0 s3 ->
+transaction_input_equiv
+(@lift_L2 AuthenticationOperation _ TD _ (File.change_owner_inner v inum))
+(@lift_L2 AuthenticationOperation _ TD _ (File.change_owner_inner v inum)) s0 s3.
+Proof.
+Transparent File.change_owner_inner.  
+Opaque Inode.get_inode.
+unfold refines_related, File.change_owner_inner; simpl; intuition eauto; cleanup.
+{
+  Transparent Inode.change_owner.
+  unfold Inode.change_owner.
+  simpl; intuition eauto.
+  {
+    Transparent Inode.get_inode.
+    simpl; unfold Inode.InodeAllocator.read; simpl; intuition eauto.
+    destruct (Compare_dec.lt_dec inum
+    Inode.InodeAllocatorParams.num_of_blocks);
+    destruct (Compare_dec.lt_dec inum
+    Inode.InodeAllocatorParams.num_of_blocks); simpl; intuition eauto.
+    solve_get_first.
+    solve_get_first.
+    unfold HC_refines in *; simpl in *; cleanup.
+    unfold TransactionToTransactionalDisk.Definitions.refines in *; simpl in *; cleanup.
+    repeat invert_lift2; cleanup.
+    eapply Transaction.read_finished in H11; eauto.
+    eapply Transaction.read_finished in H13; eauto.
+    cleanup. clear H13 H14.
+    destruct (nth_error (value_to_bits r1) inum);
+    destruct (nth_error (value_to_bits r2) inum);
+    simpl; intuition eauto.
+    destruct b, b0; simpl; intuition eauto.
+    solve_get_first.
+    solve_get_first.
+    destruct b; simpl; intuition eauto.
+    all: repeat destruct_and_split; simpl; eauto.
+    Opaque Inode.get_inode.
+  }
+
+    repeat destruct_and_split; simpl; intuition eauto.
+    {
+      repeat cleanup_pairs.
+      eapply_fresh ATC_Simulation.ATC_oracle_refines_finished in H6; eauto; cleanup.
+      eapply_fresh ATC_Simulation.ATC_oracle_refines_finished in H7; eauto; cleanup.
+      
+      eapply_fresh ATC_Simulation.ATC_exec_lift_finished in H6; eauto;
+      try solve [apply TransactionToTransactionalDisk.Refinement.TC_to_TD_core_simulation_finished];
+      try solve [apply TransactionToTransactionalDisk.Refinement.TC_to_TD_core_simulation_crashed].
+      cleanup.
+      eapply_fresh ATC_Simulation.ATC_exec_lift_finished in H7; eauto;
+      try solve [apply TransactionToTransactionalDisk.Refinement.TC_to_TD_core_simulation_finished];
+      try solve [apply TransactionToTransactionalDisk.Refinement.TC_to_TD_core_simulation_crashed].
+      cleanup.
+  
+      eapply_fresh ATC_ORS.ATC_oracle_refines_impl_eq in H2; eauto.
+      2: eapply have_same_structure_get_inode; eauto.
+      2: apply TD_oracle_refines_operation_eq.
+      cleanup.
+      repeat invert_lift2.
+      unfold AD_related_states, refines_related in *; simpl in *; cleanup.
+      unfold refines, File.files_rep, File.files_inner_rep in *; simpl in *; cleanup.
+      repeat cleanup_pairs.
+      eapply Inode.get_inode_finished in H13; eauto.
+      eapply Inode.get_inode_finished in H15; eauto.
+      cleanup; repeat split_ors; cleanup.
+      simpl in *; repeat cleanup_pairs.
+
+      unfold HC_refines in *; simpl in *; cleanup.
+      clear H19 H20.
+      unfold Inode.set_inode; simpl; intuition eauto; try congruence;
+      cleanup.
+
+      unfold Inode.InodeAllocator.write; simpl; intuition eauto.
+      destruct (Compare_dec.lt_dec inum
+      Inode.InodeAllocatorParams.num_of_blocks); try lia.
+      simpl; intuition eauto.
+      solve_get_first.
+      solve_get_first.
+
+    unfold HC_refines in *; simpl in *; cleanup.
+    unfold TransactionToTransactionalDisk.Definitions.refines in *; simpl in *; cleanup.
+    repeat invert_lift2; cleanup.
+    eapply Transaction.read_finished in H20; eauto.
+    eapply Transaction.read_finished in H24; eauto.
+    cleanup. clear H24 H27.
+    unfold HC_refines in *; simpl in *; cleanup.
+    unfold TransactionToTransactionalDisk.Definitions.refines,
+    Transaction.transaction_rep in *; simpl in *; cleanup.
+    repeat split_ors; cleanup; try congruence.
+    repeat cleanup_pairs.
+    destruct s, s3; simpl in *; try lia; eauto.
+    destruct (nth_error (value_to_bits r1) inum);
+    destruct (nth_error (value_to_bits r2) inum);
+    simpl; intuition eauto.
+    destruct b, b0; simpl; intuition eauto.
+    destruct b; simpl; intuition eauto.
+    simpl; intuition eauto.
+  }
+  unfold Inode.set_inode, Inode.InodeAllocator.write; simpl; intuition eauto.
+  destruct (Compare_dec.lt_dec inum Inode.InodeAllocatorParams.num_of_blocks); simpl; intuition eauto.
+}
+Unshelve.
+all: eauto.
+Qed.
+
+Lemma TIE_free_all_blocks:
+    forall l1 l2 s0 s3,
+refines_related ATC_Refinement
+(fun s4 s5 : state AD =>
+(exists file_block_map : disk value,
+File.DiskAllocator.block_allocator_rep
+  file_block_map (fst (snd (snd s4)))) /\ 
+(exists file_block_map : disk value,
+  File.DiskAllocator.block_allocator_rep
+    file_block_map (fst (snd (snd s5))))) s0 s3 ->
+(Transaction.get_first (fst (snd s0))
+File.DiskAllocatorParams.bitmap_addr = None <->
+Transaction.get_first (fst (snd s3))
+File.DiskAllocatorParams.bitmap_addr = None) ->
+(length (fst (snd s0)) = length (fst (snd s3))) ->
+transaction_input_equiv
+(@lift_L2 AuthenticationOperation _ TD _ (File.free_all_blocks l1))
+(@lift_L2 AuthenticationOperation _ TD _ (File.free_all_blocks l2)) s0 s3.
+Proof.
+  induction l1; destruct l2; simpl; intuition eauto.
+  {
+    unfold File.DiskAllocator.free; simpl; intuition eauto.
+    destruct (Compare_dec.lt_dec a
+    File.DiskAllocatorParams.num_of_blocks);
+    destruct (Compare_dec.lt_dec n
+    File.DiskAllocatorParams.num_of_blocks);
+    simpl; intuition eauto.
+
+    unfold AD_related_states, refines_related in *; simpl in *; cleanup.
+    unfold refines, File.files_rep in *; simpl in *; cleanup.
+    unfold HC_refines in *; simpl in *; cleanup.
+    unfold TransactionToTransactionalDisk.Definitions.refines in *; simpl in *; cleanup.
+    repeat invert_lift2; cleanup.
+    eapply Transaction.read_finished in H11; eauto.
+    eapply Transaction.read_finished in H13; eauto.
+    cleanup. clear H13 H14.
+    destruct (nth_error (value_to_bits r1) a);
+    destruct (nth_error (value_to_bits r2) n);
+    simpl; intuition eauto.
+    destruct b, b0; simpl; intuition eauto.
+    {
+      unfold AD_related_states, refines_related in *; simpl in *; cleanup.
+      unfold refines, File.files_rep in *; simpl in *; cleanup.
+      unfold HC_refines in *; simpl in *; cleanup.
+      repeat rewrite app_length, map_length in *; simpl in *.
+      erewrite addr_list_to_blocks_length_eq; try lia.
+      rewrite <- H1; eauto.
+      repeat rewrite app_length, map_length; eauto.
+    }
+    {
+      unfold AD_related_states, refines_related in *; simpl in *; cleanup.
+      unfold refines, File.files_rep in *; simpl in *; cleanup.
+      unfold HC_refines in *; simpl in *; cleanup.
+      repeat rewrite app_length, map_length in *; simpl in *.
+      erewrite addr_list_to_blocks_length_eq; try lia.
+      rewrite H1; eauto.
+      repeat rewrite app_length, map_length; eauto.
+    }
+    destruct b; simpl; intuition eauto.
+    Opaque Inode.get_all_block_numbers Inode.get_inode.
+  }
+  repeat destruct_and_split; simpl; eauto.
+  {
+    unfold AD_related_states, refines_related in *; simpl in *; cleanup.
+    unfold refines, File.files_rep in *; simpl in *; cleanup.
+    repeat cleanup_pairs.
+      eapply_fresh ATC_Simulation.ATC_oracle_refines_finished in H0; eauto; cleanup.
+      eapply_fresh ATC_Simulation.ATC_oracle_refines_finished in H4; eauto; cleanup.
+      
+      eapply_fresh ATC_Simulation.ATC_exec_lift_finished in H0; eauto;
+      try solve [apply TransactionToTransactionalDisk.Refinement.TC_to_TD_core_simulation_finished];
+      try solve [apply TransactionToTransactionalDisk.Refinement.TC_to_TD_core_simulation_crashed].
+      cleanup.
+      eapply_fresh ATC_Simulation.ATC_exec_lift_finished in H4; eauto;
+      try solve [apply TransactionToTransactionalDisk.Refinement.TC_to_TD_core_simulation_finished];
+      try solve [apply TransactionToTransactionalDisk.Refinement.TC_to_TD_core_simulation_crashed].
+      cleanup.
+  
+      eapply_fresh ATC_ORS.ATC_oracle_refines_impl_eq in H9; eauto.
+      2: eapply have_same_structure_DiskAllocator_free; eauto.
+      4: apply TD_oracle_refines_operation_eq.
+      cleanup.
+      repeat invert_lift2.
+      unfold AD_related_states, refines_related in *; simpl in *; cleanup.
+      unfold refines, File.files_rep, File.files_inner_rep in *; simpl in *; cleanup.
+      repeat cleanup_pairs.
+      eapply File.DiskAllocator.free_finished in H15; eauto.
+      eapply File.DiskAllocator.free_finished in H17; eauto.
+      cleanup; repeat split_ors; cleanup.
+      simpl in *; repeat cleanup_pairs.
+      eapply IHl1; eauto.
+      do 2 eexists; intuition eauto.
+      {
+        clear H8 H9 H12.
+        unfold File.DiskAllocator.free in *;
+        simpl in *; repeat invert_exec.
+        destruct (Compare_dec.lt_dec a
+        File.DiskAllocatorParams.num_of_blocks);
+        destruct (Compare_dec.lt_dec n
+        File.DiskAllocatorParams.num_of_blocks); try lia;
+        repeat (simpl in *; repeat invert_exec; cleanup).
+
+        unfold HC_refines in *; simpl in *; cleanup.
+        unfold TransactionToTransactionalDisk.Definitions.refines in *; simpl in *; cleanup.
+        repeat invert_lift2; cleanup.
+        eapply Transaction.read_finished in H10; eauto.
+        eapply Transaction.read_finished in H16; eauto.
+        cleanup.
+        clear H0 H9.
+        eapply Transaction.write_finished in H18; eauto.
+        eapply Transaction.write_finished in H22; eauto.
+        cleanup.
+        repeat split_ors; cleanup.
+        simpl; intuition eauto; cleanup; eauto.
+      }
+
+      {
+        clear H8 H9 H12.
+        unfold File.DiskAllocator.free in *;
+        simpl in *; repeat invert_exec.
+        destruct (Compare_dec.lt_dec a
+        File.DiskAllocatorParams.num_of_blocks);
+        destruct (Compare_dec.lt_dec n
+        File.DiskAllocatorParams.num_of_blocks); try lia;
+        repeat (simpl in *; repeat invert_exec; cleanup).
+
+        unfold HC_refines in *; simpl in *; cleanup.
+        unfold TransactionToTransactionalDisk.Definitions.refines in *; simpl in *; cleanup.
+        repeat invert_lift2; cleanup.
+        eapply Transaction.read_finished in H10; eauto.
+        eapply Transaction.read_finished in H16; eauto.
+        cleanup.
+        clear H0 H9.
+        eapply Transaction.write_finished in H18; eauto.
+        eapply Transaction.write_finished in H22; eauto.
+        cleanup.
+        repeat split_ors; cleanup.
+        simpl; intuition eauto; cleanup; eauto.
+      }
+      {
+        clear H8 H9 H12.
+        unfold File.DiskAllocator.free in *;
+        simpl in *; repeat invert_exec.
+        destruct (Compare_dec.lt_dec a
+        File.DiskAllocatorParams.num_of_blocks);
+        destruct (Compare_dec.lt_dec n
+        File.DiskAllocatorParams.num_of_blocks); try lia;
+        repeat (simpl in *; repeat invert_exec; cleanup).
+      }
+      {
+        clear H8 H9 H12.
+        unfold File.DiskAllocator.free in *;
+        simpl in *; repeat invert_exec.
+        destruct (Compare_dec.lt_dec a
+        File.DiskAllocatorParams.num_of_blocks);
+        destruct (Compare_dec.lt_dec n
+        File.DiskAllocatorParams.num_of_blocks); try lia;
+        repeat (simpl in *; repeat invert_exec; cleanup).
+
+        unfold HC_refines in *; simpl in *; cleanup.
+        unfold TransactionToTransactionalDisk.Definitions.refines in *; simpl in *; cleanup.
+        repeat invert_lift2; cleanup.
+        eapply Transaction.read_finished in H10; eauto.
+        eapply Transaction.read_finished in H17; eauto.
+        cleanup.
+        repeat split_ors; cleanup; try lia.
+        simpl in *; eauto.
+        lia.
+      }
+      
+  }
+  destruct l1; simpl; intuition eauto.
+  Unshelve.
+  all: eauto.
+Qed.
+
+Lemma free_all_blocks_transaction_content:
+forall l s u o s' r,
+exec ATCLang u o s
+(RefinementLift.compile
+   (HorizontalComposition
+      AuthenticationOperation
+      TransactionCacheOperation)
+   (HorizontalComposition
+      AuthenticationOperation
+      (TransactionalDiskLayer.TDCore
+         data_length))
+   ATCLang AD
+   (HC_Core_Refinement
+      ATCLang AD
+      Definitions.TDCoreRefinement)
+   (option unit)
+   (@lift_L2
+      AuthenticationOperation _
+      TD _ 
+      (File.free_all_blocks l)))
+(Finished s' r) ->
+(forall a, In a (map fst (fst (snd s'))) -> 
+In a (map fst (fst (snd s))) \/ a = File.DiskAllocatorParams.bitmap_addr).
+Proof.
+induction l; simpl; intros;
+  repeat invert_exec; eauto.
+eapply IHl in H1; eauto.
+unfold File.DiskAllocator.free in *; 
+repeat (simpl in *; repeat invert_exec; cleanup; eauto);
+unfold Transaction.read in *; 
+repeat (simpl in *; repeat invert_exec; cleanup; eauto);
+unfold Transaction.write in *; 
+repeat (simpl in *; repeat invert_exec; cleanup; eauto);
+repeat cleanup_pairs; intuition eauto.
+
+unfold File.DiskAllocator.free in *; 
+repeat (simpl in *; repeat invert_exec; cleanup; eauto);
+unfold Transaction.read in *; 
+repeat (simpl in *; repeat invert_exec; cleanup; eauto);
+unfold Transaction.write in *; 
+repeat (simpl in *; repeat invert_exec; cleanup; eauto);
+repeat cleanup_pairs; intuition eauto.
+Qed.
+
+Lemma get_first_some_in:
+forall (l : list (addr * value)) (a : addr)v,
+Transaction.get_first l a = Some v -> In a (map fst l).
+Proof.
+induction l; simpl; intuition eauto; try congruence.
+simpl in *; cleanup; eauto.
+Qed.
+
+
+Lemma free_all_blocks_transaction_length:
+forall l s u o s',
+exec ATCLang u o s
+(RefinementLift.compile
+   (HorizontalComposition
+      AuthenticationOperation
+      TransactionCacheOperation)
+   (HorizontalComposition
+      AuthenticationOperation
+      (TransactionalDiskLayer.TDCore
+         data_length))
+   ATCLang AD
+   (HC_Core_Refinement
+      ATCLang AD
+      Definitions.TDCoreRefinement)
+   (option unit)
+   (@lift_L2
+      AuthenticationOperation _
+      TD _ 
+      (File.free_all_blocks l)))
+(Finished s' (Some tt)) ->
+length (fst (snd s')) = length (fst (snd s)) + length l.
+Proof.
+induction l; simpl; intros;
+  repeat invert_exec; cleanup; simpl; eauto; try lia.
+
+eapply IHl in H0; eauto.
+unfold File.DiskAllocator.free in *; 
+repeat (simpl in *; repeat invert_exec; cleanup; eauto);
+unfold Transaction.read in *; 
+repeat (simpl in *; repeat invert_exec; cleanup; eauto);
+unfold Transaction.write in *; 
+repeat (simpl in *; repeat invert_exec; cleanup; eauto);
+repeat cleanup_pairs; intuition eauto.
+
+unfold File.DiskAllocator.free in *; 
+repeat (simpl in *; repeat invert_exec; cleanup; eauto);
+unfold Transaction.read in *; 
+repeat (simpl in *; repeat invert_exec; cleanup; eauto);
+unfold Transaction.write in *; 
+repeat (simpl in *; repeat invert_exec; cleanup; eauto);
+repeat cleanup_pairs; intuition eauto.
+Qed.
+
+
+Lemma TIE_delete_inner:
+forall inum u s0 s3,
+refines_related ATC_Refinement
+(fun s4 s5 : state AD =>
+ exists s1a s2a : disk File,
+ fst (snd s4) = Empty /\
+ fst (snd s5) = Empty /\
+   File.files_inner_rep s1a (fst (snd (snd s4))) /\
+   File.files_inner_rep s2a (fst (snd (snd s5))) /\
+   FD_related_states u None s1a s2a) s0 s3 ->
+transaction_input_equiv
+(@lift_L2 AuthenticationOperation _ TD _ (File.delete_inner inum))
+(@lift_L2 AuthenticationOperation _ TD _ (File.delete_inner inum)) s0 s3.
+Proof.
+  Transparent File.delete_inner.  
+  unfold refines_related, File.delete_inner; simpl; intuition eauto; cleanup.
+  {
+    Transparent Inode.get_all_block_numbers Inode.get_inode.
+    unfold Inode.get_all_block_numbers.
+    simpl; intuition eauto.
+    unfold Inode.InodeAllocator.read; simpl; intuition eauto.
+    destruct (Compare_dec.lt_dec inum
+    Inode.InodeAllocatorParams.num_of_blocks);
+    destruct (Compare_dec.lt_dec inum
+    Inode.InodeAllocatorParams.num_of_blocks); simpl; intuition eauto.
+    solve_get_first.
+    solve_get_first.
+    unfold HC_refines in *; simpl in *; cleanup.
+    unfold TransactionToTransactionalDisk.Definitions.refines in *; simpl in *; cleanup.
+    repeat invert_lift2; cleanup.
+    eapply Transaction.read_finished in H11; eauto.
+    eapply Transaction.read_finished in H13; eauto.
+    cleanup. clear H13 H14.
+    destruct (nth_error (value_to_bits r1) inum);
+    destruct (nth_error (value_to_bits r2) inum);
+    simpl; intuition eauto.
+    destruct b, b0; simpl; intuition eauto.
+    solve_get_first.
+    solve_get_first.
+    destruct b; simpl; intuition eauto.
+    all: repeat destruct_and_split; simpl; eauto.
+    Opaque Inode.get_all_block_numbers Inode.get_inode.
+  }
+    repeat destruct_and_split; simpl; intuition eauto.
+    {
+      repeat cleanup_pairs.
+      eapply_fresh ATC_Simulation.ATC_oracle_refines_finished in H0; eauto; cleanup.
+      eapply_fresh ATC_Simulation.ATC_oracle_refines_finished in H1; eauto; cleanup.
+      
+      eapply_fresh ATC_Simulation.ATC_exec_lift_finished in H0; eauto;
+      try solve [apply TransactionToTransactionalDisk.Refinement.TC_to_TD_core_simulation_finished];
+      try solve [apply TransactionToTransactionalDisk.Refinement.TC_to_TD_core_simulation_crashed].
+      cleanup.
+      eapply_fresh ATC_Simulation.ATC_exec_lift_finished in H1; eauto;
+      try solve [apply TransactionToTransactionalDisk.Refinement.TC_to_TD_core_simulation_finished];
+      try solve [apply TransactionToTransactionalDisk.Refinement.TC_to_TD_core_simulation_crashed].
+      cleanup.
+  
+      eapply_fresh ATC_ORS.ATC_oracle_refines_impl_eq in H4; eauto.
+      2: eapply have_same_structure_get_all_block_numbers; eauto.
+      2: apply TD_oracle_refines_operation_eq.
+      cleanup.
+      repeat invert_lift2.
+      unfold AD_related_states, refines_related in *; simpl in *; cleanup.
+      unfold refines, File.files_rep, File.files_inner_rep in *; simpl in *; cleanup.
+      repeat cleanup_pairs.
+      eapply Inode.get_all_block_numbers_finished in H13; eauto.
+      eapply Inode.get_all_block_numbers_finished in H15; eauto.
+      cleanup; repeat split_ors; cleanup.
+      simpl in *; repeat cleanup_pairs.
+      eapply TIE_free_all_blocks.
+      unfold refines_related; simpl; do 2 eexists; intuition eauto.
+      simpl; eexists; intuition eauto.
+      eapply File.DiskAllocator.block_allocator_rep_inbounds_eq; 
+        [| intros; FileInnerSpecs.solve_bounds ]; eauto.
+        simpl; eexists; intuition eauto.
+      eapply File.DiskAllocator.block_allocator_rep_inbounds_eq; 
+        [| intros; FileInnerSpecs.solve_bounds ]; eauto.
+      clear H H2; intuition; solve_get_first.
+      {
+        clear H H2.
+        unfold AD_related_states, refines_related in *; simpl in *; cleanup;
+        unfold refines, File.files_rep in *; simpl in *; cleanup;
+        unfold HC_refines in *; simpl in *; cleanup;
+        unfold TransactionToTransactionalDisk.Definitions.refines,
+        Transaction.transaction_rep in *; simpl in *; cleanup;
+        repeat split_ors; cleanup; try congruence;
+        repeat cleanup_pairs.
+        destruct s, s2; simpl in *; try lia; eauto.
+      }
+    }
+    repeat destruct_and_split; simpl; eauto.
+    {
+      repeat cleanup_pairs.
+      eapply_fresh ATC_Simulation.ATC_oracle_refines_finished in H0; eauto; cleanup.
+      eapply_fresh ATC_Simulation.ATC_oracle_refines_finished in H1; eauto; cleanup.
+      
+      eapply_fresh ATC_Simulation.ATC_exec_lift_finished in H0; eauto;
+      try solve [apply TransactionToTransactionalDisk.Refinement.TC_to_TD_core_simulation_finished];
+      try solve [apply TransactionToTransactionalDisk.Refinement.TC_to_TD_core_simulation_crashed].
+      cleanup.
+      eapply_fresh ATC_Simulation.ATC_exec_lift_finished in H1; eauto;
+      try solve [apply TransactionToTransactionalDisk.Refinement.TC_to_TD_core_simulation_finished];
+      try solve [apply TransactionToTransactionalDisk.Refinement.TC_to_TD_core_simulation_crashed].
+      cleanup.
+  
+      eapply_fresh ATC_ORS.ATC_oracle_refines_impl_eq in H4; eauto.
+      2: eapply have_same_structure_get_all_block_numbers; eauto.
+      2: apply TD_oracle_refines_operation_eq.
+      cleanup.
+      repeat invert_lift2.
+      unfold AD_related_states, refines_related in *; simpl in *; cleanup.
+      unfold refines, File.files_rep, File.files_inner_rep in *; simpl in *; cleanup.
+      repeat cleanup_pairs.
+      eapply Inode.get_all_block_numbers_finished in H15; eauto.
+      eapply Inode.get_all_block_numbers_finished in H17; eauto.
+      cleanup; repeat split_ors; cleanup.
+      simpl in *; repeat cleanup_pairs.
+
+
+      repeat cleanup_pairs.
+      eapply_fresh ATC_Simulation.ATC_oracle_refines_finished in H8; eauto; cleanup.
+      eapply_fresh ATC_Simulation.ATC_oracle_refines_finished in H9; eauto; cleanup.
+      
+      eapply_fresh ATC_Simulation.ATC_exec_lift_finished in H8; eauto;
+      try solve [apply TransactionToTransactionalDisk.Refinement.TC_to_TD_core_simulation_finished];
+      try solve [apply TransactionToTransactionalDisk.Refinement.TC_to_TD_core_simulation_crashed].
+      cleanup.
+      eapply_fresh ATC_Simulation.ATC_exec_lift_finished in H9; eauto;
+      try solve [apply TransactionToTransactionalDisk.Refinement.TC_to_TD_core_simulation_finished];
+      try solve [apply TransactionToTransactionalDisk.Refinement.TC_to_TD_core_simulation_crashed].
+      cleanup.
+  
+      eapply_fresh ATC_ORS.ATC_oracle_refines_impl_eq in H17; eauto.
+      (* 2: eapply have_same_structure_free_all_blocks; eauto. *)
+      3: apply TD_oracle_refines_operation_eq.
+      cleanup.
+      repeat invert_lift2.
+      unfold AD_related_states, refines_related in *; simpl in *; cleanup.
+      unfold refines, File.files_rep, File.files_inner_rep in *; simpl in *; cleanup.
+      repeat cleanup_pairs.
+      eapply FileInnerSpecs.free_all_blocks_finished in H30; eauto.
+      eapply FileInnerSpecs.free_all_blocks_finished in H32; eauto.
+      2: eapply File.DiskAllocator.block_allocator_rep_inbounds_eq; [|
+      intros; FileInnerSpecs.solve_bounds]; eauto.
+      2: eapply File.DiskAllocator.block_allocator_rep_inbounds_eq; [|
+      intros; FileInnerSpecs.solve_bounds]; eauto.
+      cleanup; repeat split_ors; cleanup.
+      simpl in *; repeat cleanup_pairs.
+
+      Transparent Inode.free.
+      unfold Inode.free, Inode.InodeAllocator.free.
+      destruct (Compare_dec.lt_dec inum
+      Inode.InodeAllocatorParams.num_of_blocks);
+      simpl; intuition eauto.
+      {
+        unfold AD_related_states, refines_related in *; simpl in *; cleanup;
+        unfold refines, File.files_rep in *; simpl in *; cleanup.
+        unfold HC_refines in *; simpl in *; cleanup.
+        unfold TransactionToTransactionalDisk.Definitions.refines,
+        Transaction.transaction_rep in H35; simpl in *; cleanup.
+        repeat split_ors; cleanup; try congruence.
+        repeat cleanup_pairs.
+        destruct s2; simpl in *; try lia.
+
+        destruct_fresh (Transaction.get_first (fst s6) Inode.InodeAllocatorParams.bitmap_addr); eauto.
+        eapply get_first_some_in in D.
+        eapply free_all_blocks_transaction_content with (a:= Inode.InodeAllocatorParams.bitmap_addr) in H9; simpl; eauto; simpl in *; intuition.
+        unfold Inode.InodeAllocatorParams.bitmap_addr,
+        File.DiskAllocatorParams.bitmap_addr in *;
+        pose proof inodes_before_data; lia.
+      }
+      {
+        unfold AD_related_states, refines_related in *; simpl in *; cleanup;
+        unfold refines, File.files_rep in *; simpl in *; cleanup.
+        unfold HC_refines in *; simpl in *; cleanup.
+        unfold TransactionToTransactionalDisk.Definitions.refines,
+        Transaction.transaction_rep in H40; simpl in *; cleanup.
+        repeat split_ors; cleanup; try congruence.
+        repeat cleanup_pairs.
+        destruct s2; simpl in *; try lia.
+
+        destruct_fresh (Transaction.get_first (fst s6) Inode.InodeAllocatorParams.bitmap_addr); eauto.
+        eapply get_first_some_in in D.
+        eapply free_all_blocks_transaction_content with (a:= Inode.InodeAllocatorParams.bitmap_addr) in H8; simpl; eauto; simpl in *; intuition.
+        unfold Inode.InodeAllocatorParams.bitmap_addr,
+        File.DiskAllocatorParams.bitmap_addr in *;
+        pose proof inodes_before_data; lia.
+      }
+      unfold HC_refines in *; simpl in *; cleanup.
+      unfold TransactionToTransactionalDisk.Definitions.refines in *; simpl in *; cleanup.
+      repeat invert_lift2; cleanup.
+      eapply Transaction.read_finished in H29; eauto.
+      eapply Transaction.read_finished in H45; eauto.
+      cleanup. clear H45 H46.
+      destruct (nth_error (value_to_bits r1) inum);
+      destruct (nth_error (value_to_bits r2) inum);
+      simpl; intuition eauto.
+      assume (A: (length (Inode.block_numbers x3) = length (Inode.block_numbers x4))).
+      destruct b, b0; simpl; intuition eauto.
+      {
+        eapply free_all_blocks_transaction_length in H8.
+        eapply free_all_blocks_transaction_length in H9.
+        repeat rewrite app_length, map_length in *;
+        simpl in *.
+        unfold AD_related_states, refines_related in *; simpl in *; cleanup.
+        unfold refines, File.files_rep in *; simpl in *; cleanup.
+        unfold HC_refines in *; simpl in *; cleanup.
+        unfold TransactionToTransactionalDisk.Definitions.refines,
+        Transaction.transaction_rep in H40, H41; simpl in *; cleanup.
+        repeat split_ors; cleanup; try congruence.
+        repeat cleanup_pairs.
+        destruct s0, s2; simpl in *; try lia.
+        setoid_rewrite A in H45.
+        erewrite addr_list_to_blocks_length_eq; eauto.
+        repeat rewrite app_length, map_length; simpl; try lia.
+        rewrite H8, H9 in *.
+        setoid_rewrite A.
+        eauto.
+      }
+      {
+        eapply free_all_blocks_transaction_length in H8.
+        eapply free_all_blocks_transaction_length in H9.
+        repeat rewrite app_length, map_length in *;
+        simpl in *.
+        unfold AD_related_states, refines_related in *; simpl in *; cleanup.
+        unfold refines, File.files_rep in *; simpl in *; cleanup.
+        unfold HC_refines in *; simpl in *; cleanup.
+        unfold TransactionToTransactionalDisk.Definitions.refines,
+        Transaction.transaction_rep in H40, H41; simpl in *; cleanup.
+        repeat split_ors; cleanup; try congruence.
+        repeat cleanup_pairs.
+        destruct s0, s2; simpl in *; try lia.
+        setoid_rewrite A.
+        erewrite addr_list_to_blocks_length_eq; eauto.
+        repeat rewrite app_length, map_length; simpl; try lia.
+        rewrite H8, H9 in *.
+        setoid_rewrite A.
+        eauto.
+      }
+      destruct b; simpl; intuition eauto.
+      {
+        eapply have_same_structure_free_all_blocks; simpl; eauto.
+
+        {
+          edestruct FileInnerSpecs.inode_exists_then_file_exists; eauto.
+          edestruct FileInnerSpecs.inode_exists_then_file_exists.
+          2: apply H27.
+          eauto.
+
+          unfold File.file_map_rep in *; cleanup.
+          eapply_fresh H31 in H29; eauto.
+          eapply_fresh H32 in H30; eauto.
+          unfold File.file_rep in *; cleanup.
+          unfold FD_related_states, same_for_user_except in *; cleanup.
+          eapply H40 in H29; eauto; cleanup; eauto.
+        }
+        eapply SameRetType.all_block_numbers_in_bound; eauto.
+        eapply File.DiskAllocator.block_allocator_rep_inbounds_eq; eauto.
+        intros; FileInnerSpecs.solve_bounds.
+
+        eapply SameRetType.all_block_numbers_in_bound.
+        4: eauto.
+        all: eauto.
+        eapply File.DiskAllocator.block_allocator_rep_inbounds_eq; eauto.
+        intros; FileInnerSpecs.solve_bounds.
+
+        {
+          eapply Forall_forall; intros.
+          eapply in_seln_exists in H29; cleanup.
+          simpl; rewrite <- H30.
+          eapply TSCommon.used_blocks_are_allocated_2; eauto.
+          eapply File.DiskAllocator.block_allocator_rep_inbounds_eq; eauto.
+          intros; FileInnerSpecs.solve_bounds.
+        }
+
+        {
+          eapply Forall_forall; intros.
+          eapply in_seln_exists in H29; cleanup.
+          simpl; rewrite <- H30.
+          eapply TSCommon.used_blocks_are_allocated_2; eauto.
+          eapply File.DiskAllocator.block_allocator_rep_inbounds_eq; eauto.
+          intros; FileInnerSpecs.solve_bounds.
+        }
+
+        {
+          unfold Inode.inode_rep, Inode.inode_map_rep,
+          Inode.inode_map_valid, Inode.inode_valid in *; cleanup.
+          eapply H39 in H27; cleanup; eauto.
+        }
+        {
+          unfold Inode.inode_rep, Inode.inode_map_rep,
+          Inode.inode_map_valid, Inode.inode_valid in *; cleanup.
+          eapply H36 in H28; cleanup; eauto.
+        }
+
+        simpl; split; eexists; eauto.
+        eapply File.DiskAllocator.block_allocator_rep_inbounds_eq; [|
+        intros; FileInnerSpecs.solve_bounds]; eauto.
+        eapply File.DiskAllocator.block_allocator_rep_inbounds_eq; [|
+        intros; FileInnerSpecs.solve_bounds]; eauto.
+      }
+    }
+    unfold Inode.free, Inode.InodeAllocator.free.
+    destruct (Compare_dec.lt_dec inum Inode.InodeAllocatorParams.num_of_blocks); simpl; intuition eauto.
+    Opaque Inode.free.
+    Unshelve.
+    all: eauto.
+    {
+          edestruct FileInnerSpecs.inode_exists_then_file_exists; eauto.
+          edestruct FileInnerSpecs.inode_exists_then_file_exists.
+          2: apply H27.
+          eauto.
+
+          unfold File.file_map_rep in *; cleanup.
+          eapply_fresh H47 in H45; eauto.
+          eapply_fresh H48 in H46; eauto.
+          unfold File.file_rep in *; cleanup.
+          unfold FD_related_states, same_for_user_except in *; cleanup.
+          eapply H56 in H45; eauto; cleanup; eauto.
+        }
 Qed.
